More examples.

test/coq/examples_simp.v
@@ -3,6 +3,9 @@ From osiris.lang Require Import lang.
 From osiris.semantics Require Import semantics evalprime. (* TODO *)
 From osiris.proofmode Require Import proofmode.
 
+Local Notation ε := EnvNil. (* TODO move *)
+Global Opaque call. (* TODO move *)
+
 (* -------------------------------------------------------------------------- *)
 
 (* An example algebraic data type. *)
@@ -19,18 +22,165 @@ Global Instance encode_data : Encode data := {
 
 (* -------------------------------------------------------------------------- *)
 
-(* let x = (A (), B ()) in let (x1, x2) = x in x1 *)
+(* let x = A() in let A() = x in () *)
 
-Definition example :=
-  ELet1Var "x" (EPair (EConstant "A") (EConstant "B")) $
-  ELet1 (PPair (PVar "x1") (PVar "x2")) (EVar "x") $
-  EVar "x1".
-
-Goal simp (eval EnvNil example) (ret (encode A)).
+Goal let e :=
+  ELet1Var "x" (EConstant "A") $
+  ELet1 (PConstant "A") (EVar "x") $
+  EUnit
+  in simp (eval ε e) (ret (encode tt)).
 Proof.
   simp.
   simp_continue.
   (* TODO why is [simp_continue] needed just once and not twice? *)
+  (* TODO same question elsewhere *)
 Qed.
 
-(* TODO Port other examples from examples_wp.v *)
+(* -------------------------------------------------------------------------- *)
+
+(* let x = (A (), B ()) in let (x1, x2) = x in x1 *)
+
+Goal let e :=
+  ELet1Var "x" (EPair (EConstant "A") (EConstant "B")) $
+  ELet1 (PPair (PVar "x1") (PVar "x2")) (EVar "x") $
+  EVar "x1"
+  in simp (eval ε e) (ret (encode A)).
+Proof.
+  simp.
+  simp_continue.
+Qed.
+
+(* -------------------------------------------------------------------------- *)
+
+(* let x = A() in y *)
+
+Goal let e :=
+  ELet1Var "x" (EConstant "A") $ EVar "y"
+  in simp (eval ε e) (ret (VConstant "A")).
+Proof.
+  (* This goal is false: the variable [y] is unbound. *)
+  simp.
+  simp_continue.
+Abort. (* expected *)
+
+(* -------------------------------------------------------------------------- *)
+
+(* let x = (z1, z2) in let (x1, x2) = x in x1 *)
+
+Goal let e :=
+  ELet1Var "x" (EPair (EVar "z1") (EVar "z2")) $
+  ELet1 (PPair (PVar "x1") (PVar "x2")) (EVar "x") $
+  EVar "x1"
+  in ∀ v1 v2,
+  let env := EnvCons "z1" v1 (EnvCons "z2" v2 ε) in
+  simp (eval env e) (ret v1).
+Proof.
+  intros.
+  simp.
+  simp_continue.
+Qed.
+
+(* -------------------------------------------------------------------------- *)
+
+(* The identity function. *)
+
+(* [identity] is an expression which returns a closure whose behavior is the
+   identity function. *)
+
+Definition identity :=
+  EFun1Var "x" (EVar "x").
+
+Definition spec_id (c : val) : Prop :=
+  ∀ v, simp (call c v) (ret v).
+
+Goal
+  ∃ c,
+  simp (eval ε identity) (ret c) ∧ spec_id c.
+Proof.
+  eexists.
+  split.
+  + simp.
+  + unfold spec_id. intros. simp_enter.
+Qed.
+
+(* -------------------------------------------------------------------------- *)
+
+(* (id (A()), id (A())) *)
+
+Goal
+  let idA := EApp (EVar "id") (EConstant "A") in
+  let e := EPair idA idA in
+  ∀ (id : val),
+  spec_id id →
+  let env := EnvCons "id" id ε in
+  simp (eval env e) (ret (VPair (VConstant "A") (VConstant "A"))).
+Proof.
+  intros ? ? id Hid ?.
+  simp.
+  (* The two components of the pair are evaluated in parallel, and
+     each of them is a function application, which is itself evaluated
+     in parallel. So we have a tree of nested [Par], which fortunately
+     is automatically simplified by [simp]. Only one [Par] remains. *)
+  eapply prove_simp_par.
+  { eapply Hid. }
+  { eapply prove_simp_bind.
+    { eapply Hid. }
+    { simp. }
+  }
+  simp.
+Qed.
+
+(* TODO *)
+
+(* The tactic [simp_specify x φ] should be used when the term begins with
+   [concatenating eval η e δ], that is, when the environment is about to be
+   extended with the environment fragment [δ].
+
+   The tactic looks up the variable [x] in the environment fragment [δ]
+   so as to find the value [v] of this variable. Then, it produces two
+   subgoals:
+   - the subgoal [φ v],
+     letting the user prove that [v] satisfies the specification [φ];
+   - the original goal,
+     generalized under the form [∀ v, φ v → ...],
+     which means that [v] becomes an opaque value
+     about which nothing is known except that [φ v] holds. *)
+
+Ltac simp_specify x φ :=
+  lazymatch goal with |- simp (concatenating eval _ _ ?δ) _ =>
+    let o := eval cbn in (lookup_name δ x) in
+    lazymatch o with ret ?v =>
+      let h := fresh in
+      assert (φ v) as H; [| revert h; generalize v ]
+    end
+  end.
+
+(* let id = identity in
+   (id (A()), id (A())) *)
+
+Goal
+  let idA := EApp (EVar "id") (EConstant "A") in
+  let e :=
+    ELet1Var "id" identity $
+    EPair idA idA
+  in simp (eval ε e) (ret (VPair (VConstant "A") (VConstant "A"))).
+Proof.
+  simp.
+  (* The environment is about to be extended with a binding of the variable
+     "id" to a certain closure. Now is the time to prove a specification
+     for this closure; then, we can make this closure opaque. *)
+  simp_specify "id" spec_id.
+  (* Subgoal: prove that the closure satisfies [spec_id]. *)
+  { unfold spec_id. intros. simp_enter. }
+  (* The variable "id" is now bound to an abstract closure [id]. *)
+  intros id Hid.
+  simp_continue.
+  (* Continue the proof as in the previous example. *)
+  eapply prove_simp_par.
+  { eapply Hid. }
+  { eapply prove_simp_bind.
+    { eapply Hid. }
+    { simp. }
+  }
+  simp.
+Qed.
